Update lexer.dfy

lexer.dfy
@@ -1,8 +1,25 @@
-include "types.dfy"
-include "validate.dfy"
+datatype TokenType = LEFT_PAREN | RIGHT_PAREN | DOT | MINUS | PLUS | STAR | SLASH 
+                     | UNARY_OP | BINARY_OP | VARIABLE_OP | NUMBER | EOF | TEMPSTRING | SPACE
 
+datatype Token = Pair(token_type:TokenType, token_value:string)
+datatype Result<T> = Ok(data: T) | Err(error: string)
 
-
+predicate validtype(token: Token){
+    token.token_type==LEFT_PAREN ||
+    token.token_type==RIGHT_PAREN ||
+    token.token_type==MINUS ||
+    token.token_type==PLUS ||
+    token.token_type==STAR ||
+    token.token_type==SLASH ||
+    token.token_type==NUMBER ||
+    token.token_type==UNARY_OP ||
+    token.token_type==BINARY_OP ||
+    token.token_type==VARIABLE_OP ||
+    token.token_type==SPACE
+}
+predicate isWhiteSpace(ch: char){
+    ch==' ' || ch=='\n' || ch=='\t'
+}
 function Flatten(tok: seq<Token>): seq<char>
 /*requires forall
 ensures |Flatten(tok)|>|tok|
@@ -41,7 +58,7 @@ function Spaceless(str: seq<char>): seq<char>
 }
 lemma SpaceAdd(ch: char,str:seq<char>)
 requires !isWhiteSpace(ch)
-ensures Spaceless(str+[ch])==Spaceless(str)+[ch]
+ensures Spaceless(str+[ch])==Spaceless(str)+[ch];
 {
 
 }
@@ -53,6 +70,7 @@ ensures Spaceless(str+tokVal)==Spaceless(str)+tokVal
     assert str+tokVal[0..i]==str;
     assert Spaceless(str)+tokVal[0..i]==Spaceless(str);
     assert Spaceless(str+tokVal[0..i])==Spaceless(str);
+    //assert tokVal[0..i]==tokVal;
     while i<|tokVal|
     invariant i<=|tokVal|
     invariant Spaceless(str)+tokVal[0..i]==Spaceless(str+tokVal[0..i])
@@ -67,11 +85,12 @@ ensures Spaceless(str+tokVal)==Spaceless(str)+tokVal
         assert Spaceless(str)+tokVal[0..i+1]==Spaceless(str+tokVal[0..i+1]);
         i:=i+1;
     }
+    assert i==|tokVal|;
     assert tokVal[0..i]==tokVal;
 }
 lemma FlatAdd(tok:seq<Token>)
     requires |tok|>=1
-    ensures Flatten(tok[0..|tok|])==Flatten(tok[0..|tok|-1])+tok[|tok|-1].token_value
+    ensures Flatten(tok[0..|tok|])==Flatten(tok[0..|tok|-1])+tok[|tok|-1].token_value;
 {
     assert tok==tok[0..|tok|];
     assert Flatten(tok)==Flatten(tok[0..|tok|]);
@@ -93,32 +112,71 @@ lemma PartialFlatAdd(i: nat, tok:seq<Token>)
 
 lemma Flatsame(tok: seq<Token>,tok2: seq<Token>)
 requires |tok|==|tok2|
-requires forall i :: 0<=i<|tok| ==> tok[i].token_value==tok2[i].token_value
+requires forall i :: 0<=i<|tok| ==> tok[i].token_value==tok2[i].token_value;
 ensures Flatten(tok)==Flatten(tok2)
 {
 
 }
-
+/*
 lemma FlatInclude(i: nat, tok:seq<Token>,str:seq<char>)
 requires Flatten(tok)==str
-//ensures exists j : nat:: 0< j < |tok[i].token_value| ==> tok[i].token_value==str[j..j+|tok[i].token_value|]
+ensures exists j : nat:: tok[i].token_value==str[j..j+|tok[i].token_value|]
 {
 
 
 }
-
+*/
 /*predicate matchesString(str: seq<char>,tokenized: seq<Token>){
     forall i :: 0<=i<|str| ==> 
     (
         
     )
 }*/
+predicate ValidUnary(tok: Token){
+    tok.token_value=="abs" || tok.token_value=="sqrt" || tok.token_value=="ceil"
+}
+predicate ValidBinary(tok: Token){
+    tok.token_value=="modulo" || tok.token_value=="expt"
+}
+predicate ValidVarOp(tok: Token){
+    tok.token_value=="min" || tok.token_value=="max"
+}
+predicate ValidString(str: seq<char>){
+    str=="abs" ||
+    str=="sqrt" ||
+    str=="ceil" ||
+    str=="modulo" ||
+    str=="expt" ||
+    str=="min" ||
+    str=="max"
 
-
+}
+predicate ValidNumber(tok: Token){
+    forall i::0<=i<|tok.token_value| ==>(
+        (tok.token_value[i] as int >=48 && tok.token_value[i] as int  <=57)
+        || tok.token_value[i]=='.'
+    )
+}
+predicate ValidWhiteSpace(tok: Token){
+    tok.token_value==" " || tok.token_value=="\n" || tok.token_value=="\t"
+}
+predicate validValue(tok: Token){
+    (tok.token_type==UNARY_OP ==> ValidUnary(tok)) &&
+    (tok.token_type==BINARY_OP ==> ValidBinary(tok)) &&
+    (tok.token_type==VARIABLE_OP ==> ValidVarOp(tok)) &&
+    (tok.token_type==NUMBER ==> ValidNumber(tok)) &&
+    (tok.token_type==PLUS ==> tok.token_value=="+") &&
+    (tok.token_type==MINUS ==> tok.token_value=="-") &&
+    (tok.token_type==STAR ==> tok.token_value=="*") &&
+    (tok.token_type==SLASH ==> tok.token_value=="/") &&
+    (tok.token_type==LEFT_PAREN ==> tok.token_value=="(") &&
+    (tok.token_type==RIGHT_PAREN ==> tok.token_value==")") &&
+    (tok.token_type==SPACE ==> ValidWhiteSpace(tok))
+}
 
 lemma validLacksSpaces(tok:Token)
-    requires validType(tok)
-    requires validValue(tok) && tok.token_type!=SPACE
+    requires validtype(tok);
+    requires validValue(tok) && tok.token_type!=SPACE;
     ensures (forall j::0<=j<|tok.token_value| ==> !isWhiteSpace(tok.token_value[j]))
 {
     /*assert tok.token_type==PLUS || tok.token_type==MINUS ||tok.token_type==STAR ||tok.token_type==SLASH ||tok.token_type==UNARY_OP ||tok.token_type==BINARY_OP ||
@@ -137,7 +195,7 @@ lemma validLacksSpaces(tok:Token)
 */
 }
 
-method lex(str: seq<char>) returns (tokenized: Result<seq<Token>>)
+method Lex1(str: seq<char>) returns (tokenized: Result<seq<Token>>)
 /*requires forall i::0<=i<|str| ==> (
 (str[i] as int >=48 && str[i] as int  <=57) ||
 str[i]=='+' ||
@@ -150,7 +208,7 @@ str[i]==')'
 
 
 
-ensures tokenized.Ok? ==> forall i:: 0<=i<|tokenized.data| ==> ((validType(tokenized.data[i])) ||tokenized.data[i].token_type==TEMPSTRING)
+ensures tokenized.Ok? ==> forall i:: 0<=i<|tokenized.data| ==> ((validtype(tokenized.data[i])) ||tokenized.data[i].token_type==TEMPSTRING)
 
 //ensures all tokens are valid and correct type
 ensures tokenized.Ok? ==> forall i:: 0<=i<|tokenized.data| ==> (
@@ -190,7 +248,7 @@ ensures tokenized.Ok? ==> Flatten(tokenized.data)==str
     //var tokpos:=0;
     var tok: seq<Token> := [];
     while i<|str|
-    invariant forall i:: 0<=i<|tok| ==> (validType(tok[i]) ||tok[i].token_type==TEMPSTRING)
+    invariant forall i:: 0<=i<|tok| ==> (validtype(tok[i]) ||tok[i].token_type==TEMPSTRING)
     invariant i<=|str|
     invariant forall i:: 0<=i<|tok| ==> (validValue(tok[i])||tok[i].token_type==TEMPSTRING)
     invariant Flatten(tok)==str[0..i]
@@ -263,9 +321,7 @@ ensures tokenized.Ok? ==> Flatten(tokenized.data)==str
             //num==0;
         }
          
-        //TODO prove this
-        //assert validType(tok[|tok|-1]) || tok[|tok|-1].token_type==TEMPSTRING;
-        assume{:axiom} validType(tok[|tok|-1]) || tok[|tok|-1].token_type==TEMPSTRING;
+        assert validtype(tok[|tok|-1]) || tok[|tok|-1].token_type==TEMPSTRING;
         assert validValue(tok[|tok|-1]);
         i:=i+1;
         
@@ -281,7 +337,7 @@ ensures tokenized.Ok? ==> Flatten(tokenized.data)==str
 method DefineTokens (oldtok: seq<Token>, str: seq<char>) returns (tokenized: Result<seq<Token>>)
 
 //ensures no tempstrings
-ensures tokenized.Ok? ==> forall i:: 0<=i<|tokenized.data| ==> (validType(tokenized.data[i]))
+ensures tokenized.Ok? ==> forall i:: 0<=i<|tokenized.data| ==> (validtype(tokenized.data[i]))
 
 //ensures all tokens are valid and correct type
 ensures tokenized.Ok? ==> forall i:: 0<=i<|tokenized.data| ==> (
@@ -289,10 +345,10 @@ ensures tokenized.Ok? ==> forall i:: 0<=i<|tokenized.data| ==> (
 )
 
 //ensures all characters are represented in order in tokens
-ensures tokenized.Ok? ==> Flatten(tokenized.data)==str
-requires forall i:: 0<=i<|oldtok| ==> (validType(oldtok[i]) || oldtok[i].token_type==TEMPSTRING)
+ensures tokenized.Ok? ==> Flatten(tokenized.data)==str;
+requires forall i:: 0<=i<|oldtok| ==> (validtype(oldtok[i]) || oldtok[i].token_type==TEMPSTRING)
 requires forall i:: 0<=i<|oldtok| ==> (validValue(oldtok[i]) || oldtok[i].token_type==TEMPSTRING)
-requires Flatten(oldtok)==str
+requires Flatten(oldtok)==str;
 
 ensures tokenized.Err? ==> (
     exists i:nat :: 
@@ -309,9 +365,9 @@ ensures tokenized.Err? ==> (
     while i<|tok|
     invariant i<=|tok|
     invariant forall j:: 0<=j<i ==> validValue(tok[j])
-    invariant forall j:: 0<=j<|tok| ==> (validType(tok[j]) ||tok[j].token_type==TEMPSTRING)
-    invariant forall j:: 0<=j<|tok| ==> (validValue(tok[j]) ||tok[j].token_type==TEMPSTRING)
-    invariant forall j:: 0<=j<i ==> ((validType(tok[j])))
+    invariant forall j:: 0<=j<|tok| ==> (validtype(tok[j]) ||tok[j].token_type==TEMPSTRING);
+    invariant forall j:: 0<=j<|tok| ==> (validValue(tok[j]) ||tok[j].token_type==TEMPSTRING);
+    invariant forall j:: 0<=j<i ==> ((validtype(tok[j])))
     invariant |a|==|tok|
     invariant forall j:: i<=j<|tok| ==> tok[j].token_type==oldtok[j].token_type
     invariant forall j:: 0<=j<|tok| ==> a[j].token_value==tok[j].token_value
@@ -322,17 +378,17 @@ ensures tokenized.Err? ==> (
         if(tok[i].token_type==TEMPSTRING){ //if token is string
             assert oldtok[i].token_type==TEMPSTRING;
             
-            if(ValidUnary(tok[i].token_value)){
+            if(ValidUnary(tok[i])){
                 tok := tok[i :=
                 Pair(UNARY_OP,tok[i].token_value)];
                 //assert validtype(tok[i]);
             }
-             else if(ValidBinary(tok[i].token_value)){
+            else if(ValidBinary(tok[i])){
                 tok := tok[i :=
                 Pair(BINARY_OP,tok[i].token_value)];
                 //assert validtype(tok[i]);
             }
-             else if(ValidVariable(tok[i].token_value)){
+            else if(ValidVarOp(tok[i])){
                 tok := tok[i :=
                 Pair(VARIABLE_OP,tok[i].token_value)];
                 //assert validtype(tok[i]);
@@ -348,7 +404,7 @@ ensures tokenized.Err? ==> (
         assert a[i].token_value==tok[i].token_value;
         Flatsame(tok,a);
         assert tok[i].token_type!=TEMPSTRING;
-        assert validType(tok[i]);
+        assert validtype(tok[i]);
         //assert tok[i].token_type==UNARY_OP ==> ValidUnary(tok[i]);
         i:=i+1;
     }
@@ -357,12 +413,15 @@ ensures tokenized.Err? ==> (
 
 
 
-method RemoveSpaces(tok: seq<Token>) returns (spaceless: seq<Token>)
+method RemoveSpaces(tok: seq<Token>) returns (spaceless: Result<seq<Token>>)
 //requires forall i:: 0<=i<|tok| ==> (forall j::0<=j<|tok[i].token_value| ==> !isWhiteSpace(tok[i].token_value[j]))
 requires forall i:: 0<=i<|tok| ==> (validValue(tok[i]))
-requires forall i:: 0<=i<|tok| ==> (validType(tok[i]))
-ensures forall i:: 0<=i<|spaceless| ==> spaceless[i].token_type!=SPACE
-ensures Flatten(spaceless)==Spaceless(Flatten(tok))
+requires forall i:: 0<=i<|tok| ==> (validtype(tok[i]))
+ensures spaceless.Ok?
+ensures forall i:: 0<=i<|spaceless.data| ==> (validValue(spaceless.data[i]))
+ensures forall i:: 0<=i<|spaceless.data| ==> (validtype(spaceless.data[i]))
+ensures forall i:: 0<=i<|spaceless.data| ==> spaceless.data[i].token_type!=SPACE
+ensures Flatten(spaceless.data)==Spaceless(Flatten(tok))
 {
     var i:=0;
     var out: seq<Token> := [];
@@ -370,7 +429,9 @@ ensures Flatten(spaceless)==Spaceless(Flatten(tok))
     //assert forall i:: 0<=i<|tok| ==> (forall j::0<=j<|tok[i].token_value| ==> !isWhiteSpace(tok[i].token_value[j]));
     while i<|tok|
     invariant i<=|tok|
-    invariant forall j::0<=j<|out| ==> out[j].token_type!=SPACE
+    invariant forall i:: 0<=i<|tok| ==> (validValue(tok[i]))
+    invariant forall i:: 0<=i<|tok| ==> (validtype(tok[i]))
+    invariant forall j::0<=j<|out| ==> (out[j].token_type!=SPACE && validValue(out[j]) && validtype(out[j]))
     invariant Flatten(out)==Spaceless(Flatten(tok[0..i]))
     {
         
@@ -400,10 +461,52 @@ ensures Flatten(spaceless)==Spaceless(Flatten(tok))
     }
     assert i==|tok|;
     assert tok[0..|tok|]==tok;
-    return out;
+    return Ok(out);
 }
 
+method Lex (str:seq<char>)returns (tokenized: Result<seq<Token>>)
+ensures tokenized.Ok? ==> forall i:: 0<=i<|tokenized.data| ==> ((validtype(tokenized.data[i])))
 
+//ensures all tokens are valid and correct type
+ensures tokenized.Ok? ==> forall i:: 0<=i<|tokenized.data| ==> (
+    validValue(tokenized.data[i])
+)
+
+//ensures all characters are represented in order in tokens
+
+
+//ensures no false positives when returning errors
+/*ensures tokenized.Err? ==> (
+
+(exists i: nat:: i<|str| && !(
+    ((str[i] as int >=48 && str[i] as int  <=57) || str[i]=='.') ||
+    (str[i] as int >=97 && str[i] as int  <=122) ||
+    str[i]=='+' ||
+    str[i]=='-' ||
+    str[i]=='*' ||
+    str[i]=='/' ||
+    str[i]=='(' ||
+    str[i]==')' ||
+    (str[i]==' ' || str[i]=='\n' || str[i]=='\t')
+))
+)*/
+
+
+//ensures tokenized.Ok? ==> Flatten(tokenized.data)==str
+{
+    var tok:= Lex1(str);
+    if(tok.Ok?){
+        tok:=DefineTokens(tok.data,str);
+        if(tok.Ok?){
+            tok:=RemoveSpaces(tok.data);
+            return tok;
+        }
+        return tok;
+    }
+    return tok;
+
+
+}
 
 /*match result_var
            case Ok => do something;
